Implemented missing evalRelB iter case.
Started repeat formalization with syntax.
Developed a proof for equivalence of evalB and eval.
Added some documentation for boolean evaluations.

Logic/DL/FinModelSemantics.lean
@@ -1,11 +1,9 @@
 import Logic.DL.Semantics
-import Mathlib.Data.Fintype.Basic
-import Mathlib.Data.Finset.Basic
 
 namespace Logic.DL
 
 
---helpers to extract states and relations directly
+--helpers to extract states and relations directly from transition list
 def relsFromList
   {RelType State: Type}
   [BEq RelType]
@@ -33,6 +31,11 @@ def relFromList
   RelType → State → State → Prop :=
     λ relAtom s₁ s₂ ↦ (relAtom, s₁, s₂) ∈ rels
 
+/-- Constructs a kripke model `M` from explicit valuation and relation lists:
+* `valList: List (AtomType × State)` specifies `M.val` where a tuple `(a, s)` defines `a` holds at `s`
+
+• `relList: List (RelType × State × State)` specifies `M.rel` where a triple `(r, s, s')` defines a transition s --r--> s'
+-/
 def mkModel
   {RelType AtomType State: Type}
   [DecidableEq RelType] [DecidableEq AtomType] [DecidableEq State]
@@ -64,10 +67,54 @@ def relDecidable
     simp[relFromList]
     infer_instance
 
+
+mutual --mutual block needed since successorStates, relBFS and evalRelB depend on each other
+
+-- helper to get states reachable via one α step
+def successorStates
+  {RelType AtomType State: Type}
+  [DecidableEq RelType] [DecidableEq State]
+  (M: KripkeModel RelType AtomType State)
+  (relDecidableH: ∀ rel s s', Decidable (M.rel rel s s'))
+  (states: List State) (rels: List RelType)
+  (α: Relation RelType) (s: State): List State :=
+    states.filter (λ s' ↦ evalRelB M relDecidableH states rels α s s')
+
+def relBFS
+  {RelType AtomType State: Type}
+  [DecidableEq RelType] [DecidableEq State]
+  (M: KripkeModel RelType AtomType State)
+  (relDecidableH: ∀ rel s s', Decidable (M.rel rel s s'))
+  (states: List State) (rels: List RelType)
+  (α: Relation RelType)
+  (maxSteps: Nat) (fringe visited: List State) (target: State): Bool :=
+    if target ∈ fringe then Bool.true
+    else
+      match maxSteps with
+        | 0 => false
+        | maxSteps' + 1 =>
+          let next := fringe
+                        |>.map (λ s ↦ (successorStates M relDecidableH states rels α s))
+                        |>.flatten
+                        |>.eraseDups
+                        |>.filter (λ s ↦ !(s ∈ visited))
+          relBFS M relDecidableH states rels α maxSteps' next (visited ++ next) target
 /-
-Boolean evaluation logic for finite models
+# Boolean evaluation logic for finite models
 -/
 
+
+/-- Boolean evaluation of a relation `α` between states `s₀` and `s₁` in a finite kripke model `M`
+
+`evalRelB` is computational, i.e. it evaluates relation semantics to `Bool` using decidability of `M.rel` supplied via `relDecidableH` argument.
+This Decidable instance can ge generated using `Logic.DL.relDecidable`.
+The evaluation is inductively extended to non-atomic relations.
+
+Explicit lists `List State` and `List RelType` containing states and atomic relations have to be provided.
+`evalRelB` is intended for computation over a finite model rather than reasoning. For general reasoning, use `Logic.DL.evalRel` instead.
+### Returns
+`Bool.true` iff `α` is a transition between `s₀` and `s₁` in `M`, `Bool.false` otherwise.
+-/
 def evalRelB
   {RelType AtomType State: Type}
   [DecidableEq RelType] [DecidableEq State]
@@ -84,8 +131,22 @@ def evalRelB
                                                   evalRelB M relDecidableH states rels β s₂ s₁)
   | Relation.alt α β, s₀, s₁ => evalRelB M relDecidableH states rels α s₀ s₁ ||
                                 evalRelB M relDecidableH states rels β s₀ s₁
-  | Relation.iter α, s₀, s₁ => decide (s₀ = s₁) --reflexive only → TODO: implement transitive!
+  | Relation.iter α, s₀, s₁ => relBFS M relDecidableH states rels α states.length [s₀] [s₀] s₁
 
+end --end mutual block
+
+
+/-- Boolean evaluation of a formula `φ` at a state `s` in a finite kripke model `M`
+
+`evalB` is computional, i.e. it evaluates propositions of `AtomType` to `Bool` using decidability of `M.rel`, `M.val` supplied via `relDecidableH`, `valDecidableH` args.
+These Decidable instances can be generated using `Logic.DL.relDecidable` and `Logic.DL.valDecidable`.
+The evaluation is inductively extended to non-atomic formulas.
+
+Explicit lists `List State` and `List RelType` containing states and atomic relations have to be provided.
+`evalB` is intended for computation over a finite model rather than reasoning. For general reasoning, use `Logic.DL.eval` instead.
+### Returns
+`Bool.true` iff M, s ⊧ φ, `Bool.false` otherwise.
+-/
 def evalB
   {RelType AtomType State: Type}
   [DecidableEq RelType] [DecidableEq State]
@@ -94,7 +155,7 @@ def evalB
   (valDecidableH: ∀ atom s, Decidable (M.val atom s))
   (states: List State) (rels: List RelType):
   DLForm RelType AtomType → State → Bool
-  
+
   | DLForm.atom a, s => @decide (M.val a s) (valDecidableH a s)
   | DLForm.falsum, _ => false
   | DLForm.imp φ ψ, s => (! evalB M relDecidableH valDecidableH states rels φ s) ||
@@ -103,8 +164,17 @@ def evalB
                                               evalRelB M relDecidableH states rels α s s' &&
                                               evalB M relDecidableH valDecidableH states rels φ s')
 
+/-- Wrapper to evaluate a formula `φ` at state `s` in a finite kripke model `M` constructed from explicit valuation and relations list.
 
---wrapper to evaluate directly over model defining rel/val in list notation
+The modle `M` is not given directly, but inferred from:
+* `vals: List (AtomType × State)` specifies which atomic propositions hold in specific states
+* `rels: List (RelType × State × State)` specifies atomic state transitions
+
+States and atomic relations are inferred from these lists and the resulting model is passed to `evalB`
+
+### Returns
+`Bool.true` iff M, s ⊧ φ, `Bool.false` otherwise
+-/
 def evalFromList
   {RelType AtomType State: Type}
   [DecidableEq RelType] [DecidableEq AtomType] [DecidableEq State]
