Main.lean
@@ -29,21 +29,22 @@ end
 
 namespace Logic.DL
 
-abbrev State := List DynamicIndices --use List of dynamic indices where [0, 1] corresponds to 0.1
+abbrev State := List DynamicIdxSym --use List of dynamic indices where [0, 1] corresponds to 0.1
 
 
 def val: List (Atoms × State) :=
   [ ("q", []),
     ("p", [0]),
     ("q", [0, 1]),
-    ("p", [0, 1])] -- "in state 0.1 p holds"
+    ("p", [0, 1]), -- "in state 0.1 p holds"
+    ("r", [0, 1, #])]
 
-def rel: List (DynamicIndices × State × State) :=
+def rel: List (DynamicIdxSym × State × State) :=
   [ (0, [], [0]), -- [] --0--> [0]
     (1, [0], [0, 1]), -- [0] --1--> [0, 1]/0.1
     (#, [0, 1], [0, 1, #])]
 
-def M₁: KripkeModel DynamicIndices Atoms State :=
+def M₁: KripkeModel DynamicIdxSym Atoms State :=
   mkModel val rel
 
 
@@ -59,16 +60,18 @@ def rels := relsFromList rel
 #eval evalB M₁ relH valH states rels (⟨0⟩ "p") []
 #eval evalB M₁ relH valH states rels ("p") []
 
-#eval evalFromList val rel (⟨0⟩ "p") []
-#eval evalFromList val rel (⟨0 ∪ 1⟩("p" ∧ "q")) []
-#eval evalFromList val rel (⟨0 ∪ 1⟩("p" ∧ "q")) [0]
-#eval evalFromList val rel ((⟨Relation.comp 0 (Relation.comp 1 •)⟩¬⊥)) []
+#eval evalFromList val rel (⟨0 1⟩ "p") []
+#eval evalFromList val rel (⟨0 ∪ 1⟩("p" ⋏ "q")) []
+#eval evalFromList val rel (⟨0 ∪ 1⟩("p" ⋏ "q")) [0]
+#eval evalFromList val rel ((⟨0 1 •⟩ ∼⊥)) []
+#eval evalFromList val rel (⟨•*⟩ "r") []
+#eval evalFromList val rel (⟨0*⟩ "r") []
 
 def val': List (Atoms × State) :=
   [ ("p", [0]),
     ("q", [1])
   ]
-def rel': List (DynamicIndices × State × State) :=
+def rel': List (DynamicIdxSym × State × State) :=
   [ (0, [], [0]),
     (0, [], [1]) --branching
   ]
@@ -76,9 +79,27 @@ def rel': List (DynamicIndices × State × State) :=
 #eval evalFromList val' rel' (⟨0 ∪ 1⟩"p") []
 #eval evalFromList val' rel' (⟨•⟩ "p") []
 #eval evalFromList val' rel' ([•] "q") []
-#eval evalFromList val' rel' ((⟨0⟩ "p") ∧ (⟨0⟩ ¬ "p")) [] --true due to branching model
+#eval evalFromList val' rel' ((⟨0⟩ "p") ⋏ (⟨0⟩ ∼"p")) [] --true due to branching model
 #eval evalFromList val' rel' (⟨•⟩ "q") []
-#eval evalFromList val' rel' (⟨0⟩ "p" ∧ "q") []
-#eval evalFromList val' rel' (⟨0⟩ ¬("p" ∨ "q")) []
+#eval evalFromList val' rel' (⟨0⟩ "p" ⋏ "q") []
+#eval evalFromList val' rel' (⟨0⟩ ∼("p" ⋎ "q")) []
 
+
+def val'': List (Atoms × State) :=
+  [ ("p", [6])]
+
+def rels'': List (DynamicIdxSym × State × State) :=
+  [ (0, [], [0]),
+    (0,[0], [0, 0]),
+    (0, [0, 0], [0, 1]),
+    (0, [0, 1], [0, 2]),
+    (0, [0, 2], [1]),
+    (1, [1], [6]),
+    (1, [6], [])
+  ]
+
+#eval evalFromList val'' rels'' (⟨(0*) 1*⟩"p") []
+#eval evalFromList val'' rels'' ([1*]"p") []
+#eval evalFromList val'' rels'' (⟨(0 ∪ 1)*⟩"p") []
+#eval evalFromList val'' rels'' (⟨•*⟩ "p") []
 end Logic.DL
