Logic/DL/Notation.lean
@@ -3,31 +3,33 @@ namespace Logic.DL
 
 /-
 # Remarks
-- This approach is only applicable when using the monomorphic DAForm, which fixes DynamicIndices and Atoms as DLForm Types
-- Any non atomic formula has to be parenthesized in order to ensure correct precedence - TODO!
-- Whitespaces need to be present between composition operator "." and the operands when using Nats, otherwise parsed as single number
+- This approach is only applicable when using the monomorphic DAForm, which fixes DynamicIndices and Atoms as DLForm Types.
+- In order to avoid confusion with Leans inbuilt notation for Props, the following logical connectives have to be chosen slightly different than usual textbook:
+  • `⋎` for DL "or"
+  • `⋏` for DL "and"
+  • `∼` for DL "not"
 -/
 
 
 -- relevant coercions
-instance: Coe DynamicIndices (Relation DynamicIndices) where
+instance: Coe DynamicIdxSym (Relation DynamicIdxSym) where
   coe α := Relation.relAtom α
 
-instance: OfNat DynamicIndices n where
-  ofNat := DynamicIndices.line n
+instance: OfNat DynamicIdxSym n where
+  ofNat := DynamicIdxSym.line n
 
-instance: OfNat (Relation DynamicIndices) n where
-  ofNat := Relation.relAtom (DynamicIndices.line n)
+instance: OfNat (Relation DynamicIdxSym) n where
+  ofNat := Relation.relAtom (DynamicIdxSym.line n)
 
-instance: Coe String (DLForm DynamicIndices Atoms) where
+instance: Coe String (DLForm DynamicIdxSym Atoms) where
   coe p := DLForm.atom (Atoms.name p)
 
 instance: Coe String Atoms where
   coe p := Atoms.name p
 
 --basic notations
-notation "$" => DynamicIndices.dollar
-notation "#" => DynamicIndices.hash
+notation "$" => DynamicIdxSym.dollar
+notation "#" => DynamicIdxSym.hash
 
 notation "∅" => Relation.emptyset
 notation "•" => Relation.wild
@@ -36,27 +38,31 @@ notation "⊥" => DLForm.falsum
 
 
 --relation operators
-notation:80 α " . " β  => Relation.comp (α: Relation DynamicIndices) (β: Relation DynamicIndices)
-notation:70 α " ∪ " β => Relation.alt (α: Relation DynamicIndices) (β: Relation DynamicIndices)
-notation:max α "*" => Relation.iter (α: Relation DynamicIndices)
+notation:max α "*" => Relation.iter (α: Relation DynamicIdxSym)
+notation:80 α:81 β:80 => Relation.comp (α: Relation DynamicIdxSym) (β: Relation DynamicIdxSym)
+notation:70 α:71 " ∪ " β:70 => Relation.alt (α: Relation DynamicIdxSym) (β: Relation DynamicIdxSym)
 
 --formulas
-abbrev DAForm := DLForm DynamicIndices Atoms
-
-notation:60 φ " → " ψ => DLForm.imp (φ: DAForm) (ψ: DAForm)
-notation:90 "⟨" α "⟩" φ => DLForm.diamond (α: Relation DynamicIndices) (φ: DAForm)
-notation:90 "[" α "]" φ => box (α: Relation DynamicIndices) (φ: DAForm)
-notation:85 "¬" φ => not (φ: DAForm)
-notation:70 φ " ∧ " ψ => conj (φ: DAForm) (ψ: DAForm)
-notation:65 φ " ∨ " ψ => disj (φ: DAForm) (ψ: DAForm)
+abbrev DAForm := DLForm DynamicIdxSym Atoms
 
 
-#check [(0)*] "p"
-#check ¬⟨0 . $⟩ ¬"p" ∧ "q"
-#check ¬⟨0 . #⟩ (¬ "p") ∧ "q"
-#check "p" ∨ "q" ∧ "p"
-#check ("p" ∧ "q") ∨ "p"
-#check "p" ∧ ⊥ ∨ "p"
+notation:90 "⟨" α "⟩" φ => DLForm.diamond (α: Relation DynamicIdxSym) (φ: DAForm)
+notation:90 "[" α "]" φ => box (α: Relation DynamicIdxSym) (φ: DAForm)
+notation:85 "∼" φ:85 => not (φ: DAForm)
+notation:70 φ:71 " ⋏ " ψ:70 => conj (φ: DAForm) (ψ: DAForm)
+notation:60 φ:61 " ⋎ " ψ:60 => disj (φ: DAForm) (ψ: DAForm)
+notation:50 φ:51 " → " ψ:50 => DLForm.imp (φ: DAForm) (ψ: DAForm)
+
+
+#check 0 1 2 3 #
+#check [(0 1 * ∪ 1)*] "p"
+#check 0 ∪ 1 * ∪ #
+#check ∼ ⟨0 $⟩   ∼ "p" ⋎ "q" --
+#check ∼⟨0 #⟩ (∼ "p") ⋎ "q"
+#check "p" ⋎ "q" ⋏ "p"
+#check "p" ⋏ "q" ⋎ "p"
+#check "p" ⋏ ⊥ ⋎ "p"
+#check "p" ⋎ "p" ⋎ "p" ⋏ "q" ⋎ "q"
 #check "p" → "q"
 #check ⊥
 #check #
