Logic/DL/Proofs.lean
@@ -1,10 +1,10 @@
 import Logic.DL.Semantics
-
+import Logic.DL.FinModelSemantics
 namespace Logic.DL
 
 open DLForm
 open Relation
-set_option trace.Meta.Tactic.simp.rewrite true
+--set_option trace.Meta.Tactic.simp.rewrite true
 
 --formulas are equivalent to themselves
 theorem equiv_refl{RelType AtomType State: Type} (φ: DLForm RelType AtomType):
@@ -43,5 +43,91 @@ theorem wild_imp_ato (M: KripkeModel RelType AtomType State):
   intro h
   simp[evalRel] at *
   exact h
+
+theorem evalRelB_correct
+  {RelType AtomType State: Type}
+  [DecidableEq RelType] [DecidableEq State]
+  (M: KripkeModel RelType AtomType State)
+  (relDecidableH: ∀ rel s s', Decidable (M.rel rel s s'))
+  (states: List State) (rels: List RelType)
+  (α: Relation RelType) (s₀ s₁: State):
+    evalRelB M relDecidableH states rels α s₀ s₁ = Bool.true ↔ evalRel M α s₀ s₁ :=
+    sorry
+
+
+/- Correctness proof for evalB under assumptions:
+  • evalRelB is correct
+  • all states are passed in states: List State
+ -/
+theorem evalB_correct
+  {RelType AtomType State: Type}
+  [DecidableEq RelType] [DecidableEq State]
+  (M: KripkeModel RelType AtomType State)
+  (relDecidableH: ∀ rel s s', Decidable (M.rel rel s s'))
+  (valDecidableH: ∀ atom s, Decidable (M.val atom s))
+  (states: List State) (rels: List RelType)
+  (φ: DLForm RelType AtomType)
+  (allStatesPassedH: ∀ α s s', evalRel M α s s' → s' ∈ states):
+    ∀ s, evalB M relDecidableH valDecidableH states rels φ s = Bool.true ↔ eval M φ s :=
+    by
+      induction φ with
+        | atom => simp[evalB, eval]
+        | falsum => simp[evalB, eval]
+        | imp φ ψ ihφ ihψ =>  simp[evalB, eval, ihψ]
+                              intro s
+                              constructor
+                              · intro evalBH
+                                intro evalφh
+                                have hbφ := (ihφ s).mpr evalφh
+                                cases evalBH with
+                                  | inl hnotbφ =>
+                                      have cont: Bool.true = false :=
+                                        by rw [hbφ] at hnotbφ; exact hnotbφ
+                                      cases cont -- cont has no constructor -> done
+                                  | inr hψ => exact hψ
+                              · intro evalH
+                                cases evalBH: evalB M relDecidableH valDecidableH states rels φ s with
+                                  | false => apply Or.inl; rfl
+                                  | true => apply Or.inr
+                                            have hφ := (ihφ s).mp evalBH
+                                            apply evalH hφ
+
+        | diamond α φ ihφ =>  simp[evalB, eval]
+                              intro s
+                              constructor
+                              · intro evalBH
+                                --split evalBH
+                                cases evalBH with
+                                  | intro s' inner =>
+                                    cases inner with
+                                      | intro sInStates evalBSemH
+
+                                    have evalαH: evalRel M α s s' :=
+                                      ((evalRelB_correct M relDecidableH states rels α s s').mp evalBSemH.left)
+                                    have evalφH: eval M φ s' :=
+                                      ((ihφ s').mp evalBSemH.right)
+
+                                    apply Exists.intro s'
+                                    apply And.intro
+                                    · exact evalαH
+                                    · exact evalφH
+
+                              · intro evalH
+                                cases evalH with
+                                  | intro s' inner =>
+                                    cases inner with
+                                      | intro evalαH evalφH
+                                    have s'InStatesH: s' ∈ states := allStatesPassedH α s s' evalαH --correctness relies on passing all states to evalB, i.e. that s' ∈ states
+
+                                    have evalαBH: evalRelB M relDecidableH states rels α s s' :=
+                                      ((evalRelB_correct M relDecidableH states rels α s s').mpr evalαH)
+
+                                    have evalφBH: evalB M relDecidableH valDecidableH states rels φ s' :=
+                                      (ihφ s').mpr evalφH
+
+                                    apply Exists.intro s'
+                                    apply And.intro
+                                    · exact s'InStatesH
+                                    · apply And.intro evalαBH evalφBH
 
 end Logic.DL
