Logic/REPEAT/Syntax.lean
@@ -1,0 +1,87 @@
+namespace Logic.REPEAT
+
+
+--Variables
+inductive Var: Type
+  | name: String → Var
+deriving DecidableEq, BEq
+
+
+/-
+Expressions
+TODO: Design choice - keep Expressions and Conditions seperated?
+-/
+
+inductive Expr: Type
+  | const: Int → Expr                 --constant integers
+  | access: Var → Expr → Expr         --variable access `v[e]`
+  | sub: Expr → Expr → Expr           --subtraction `e₀ - e₁`
+  | le: Expr → Expr → Expr            --condition `e₀ ≤ e₁`
+deriving DecidableEq, BEq
+
+-- Arguments
+inductive Arg: Type
+  | var: Var → Arg                   --call by value
+  | ref: Var → Arg                   --call by name
+deriving DecidableEq, BEq
+
+--Statements
+inductive Stmt: Type
+  | call: Expr → List Arg → Stmt    --`call INT_PROC_ID (args*)`
+  | assign: Var → Expr → Expr → Stmt --assignment `v[e₀] = e₁`
+  | returnIf: Expr → Stmt            --conditional return `if e₀ return`
+deriving DecidableEq, BEq
+
+--enumerated statements, i.e. carrying line number
+structure LStmt where
+  line: Nat                           --line number
+  stmt: Stmt                          --statement
+
+--Procedures
+structure Proc where
+  id: Int                             --proc id
+  params: List Var                    --formal parameters of a procedure
+  body: List LStmt                    --procedure body as a list of numbered stmts
+  loops: Bool                         --flag for repeat keyword
+
+--Programs are just lists of procedures
+abbrev Program := List Proc
+
+
+--Syntactic sugar
+namespace Expr
+
+--variable shorthand `x = x[0]`
+def var (v: Var) : Expr :=
+  access v (const 0)
+
+
+--boolean constants
+def TRUE : Expr := const 1
+def FALSE: Expr := const 0
+
+--unary minus
+def unMin (e: Expr): Expr := sub (const 0) e
+
+--addition
+def add (e₀ e₁: Expr): Expr := sub e₀ (unMin e₁)
+
+
+/-
+Derived boolean operators. As of right now, there is nothing enforcing the operands are only 0/1
+- see TODO design choice for expressions
+-/
+-- ¬c := c ≤ 0
+def not (c: Expr): Expr := le c (const 0)
+
+-- c₀ ∨ c₁ := ¬c₀ ≤ c₁
+def disj (c₀ c₁: Expr): Expr := le (not c₀) c₁
+
+-- c₀ ∧ c₁ := ¬(c₀ ≤ ¬c₁)
+def conj (c₀ c₁: Expr): Expr := not (le c₀ (not c₁))
+
+-- e₀ == e₁ := e₀ ≤ e₁ ∧ e₁ ≤ e₀
+def eq (e₀ e₁: Expr): Expr := conj (le e₀ e₁) (le e₁ e₀)
+
+end Expr
+end Logic.REPEAT
